thys/Ordinary_Differential_Equations/Ex/Lorenz/Lorenz_C0.thy
@@ -4,6 +4,6 @@ theory Lorenz_C0
 begin
 
 lemma check_lines_c0: "check_lines False ordered_lines"
-  by (parallel_check (* "output/lorenz_c0_" *) "" 15 9)
+  by (parallel_check (* "output/lorenz_c0_" *) _ 15 9)
 
 end
